tests/demo/A_hpp_proof.v
@@ -1,0 +1,44 @@
+Require Import Coq.ZArith.BinInt.
+Require Import Coq.Strings.String.
+
+Local Open Scope Z_scope.
+Local Open Scope string_scope.
+
+From ChargeCore.Logics Require Import
+     ILogic BILogic ILEmbed Later.
+
+Require Import Cpp.Parser.
+Require Import Cpp.HoareSemantics.
+Require Import auto.Tactics.Discharge.
+
+Require Demo.A_hpp.
+Require Import Demo.A_hpp_spec.
+
+
+
+Opaque denoteModule.
+
+(* soundness of the specification *)
+Theorem A_hpp_sound : forall (resolve : genv),
+    denoteModule nil A_hpp.module |-- A_hpp_spec resolve.
+Proof.
+  intros.
+  simpl.
+  unfold A_hpp_spec.
+  work.
+  eapply verify_func.
+  { (* todo(gmm): make this reflective *)
+    repeat econstructor. }
+  unfold  func_ok'. simpl.
+  work.
+  simplifying.
+  repeat perm_left ltac:(idtac; perm_right ltac:(idtac; eapply wp_call_glob)).
+  simplifying.
+  unfold tlocal, tptsto.
+  work. subst.
+  simplifying.
+  generalize (has_type_int_bound H1). intro.
+  work.
+  simplifying.
+  work.
+Qed.
