tests/demo/A_hpp_spec.v
@@ -1,0 +1,38 @@
+Require Import Coq.ZArith.BinInt.
+Require Import Coq.Strings.String.
+
+Local Open Scope Z_scope.
+Local Open Scope string_scope.
+
+From ChargeCore.Logics Require Import
+     ILogic BILogic ILEmbed Later.
+
+Require Import Cpp.Parser.
+Require Import Cpp.HoareSemantics.
+Require Demo.A_hpp.
+
+Definition A__foo := {| g_path := "A" :: NStop ; g_name := "foo" |}.
+Definition A__foo_spec : function_spec' :=
+  ht' (Qmut T_int) (Qmut T_int :: nil)
+      (fun x =>
+         {| wpp_with := Z
+          ; wpp_pre := fun y => [| x = Vint y |] ** [| 0- 2^31 < (y + 6)%Z < 2^31 -1 |]
+          ; wpp_post := fun y (r : val) => [| r = Vint (y + 6)%Z |]
+          |}).
+
+Definition A__bar := {| g_path := "A" :: NStop ; g_name := "bar" |}.
+Definition A__bar_spec : function_spec' :=
+  ht' (Qmut T_int) (Qmut T_int :: nil)
+      (fun x =>
+         {| wpp_with := Z
+          ; wpp_pre := fun y => [| x = Vint y |] ** [| 0- 2^31 < (y + 7)%Z < 2^31 -1 |]
+          ; wpp_post := fun y (r : val) => [| r = Vint (y + 7)%Z |]
+          |}).
+
+Definition A_hpp_spec (resolve : _) :=
+      (|> cglob' (resolve:=resolve) A__foo A__foo_spec) -* cglob' (resolve:=resolve) A__bar A__bar_spec.
+
+
+(* this is an axiom *)
+Axiom has_type_int_any : forall x, has_type (Vint x) T_int.
+Axiom has_type_int_bound : forall {q x}, has_type (Vint x) (Tqualified q T_int) -> -(2^31) < x < 2^31 - 1.
