tests/demo/A_o.v
@@ -1,0 +1,50 @@
+From Cpp Require Import
+     Ast HoareSemantics.
+From ChargeCore.Logics Require Import
+     ILogic BILogic ILEmbed Later.
+
+From Demo Require
+     A_hpp A_hpp_spec A_hpp_proof
+     A_cpp A_cpp_spec A_cpp_proof.
+Import A_hpp_spec.
+
+Definition module_link (a b : list Decl) : list Decl := a ++ b.
+
+Axiom denoteModule_link : forall nss a b,
+    denoteModule nss (module_link a b) -|- denoteModule nss a ** denoteModule nss b.
+
+(* todo(gmm): I'm a bit confused about the appropriate specification of linking
+ *)
+Lemma wand_apply : forall A B : mpred,
+    A |-- (A -* B) ** B.
+Proof.
+  intros.
+Abort.
+
+Lemma lob_link : forall A B : mpred,
+    ((|> A) -* B) ** ((|> B) -* A) |-- A ** B.
+Proof.
+  intros.
+  eapply sepSPAdj'.
+  rewrite <- empSPL.
+  eapply sepSPAdj.
+  rewrite <- (landtrueR empSP).
+  apply landL2.
+  eapply spec_lob.
+Abort.
+    (* |>A ==> B
+     * |>B ==> A
+     * A //\\ B
+     *)
+
+Theorem A_o_sound (resolve : _)
+: denoteModule nil (module_link A_hpp.module A_cpp.module)
+  |-- cglob' (resolve:=resolve) A__foo A__foo_spec **
+      cglob' (resolve:=resolve) A__bar A__bar_spec.
+Proof.
+  rewrite denoteModule_link.
+  rewrite (A_cpp_proof.A_cpp_sound resolve).
+  rewrite (A_hpp_proof.A_hpp_sound resolve).
+  unfold A_hpp_spec.
+  unfold A_cpp_spec.A_cpp_spec.
+Abort. (* todo(gmm): finish this proof *)
